lib/nicta_lib/clib/CCorresLemmas.thy
@@ -20,7 +20,7 @@ lemma ccorres_rel_imp2:
   apply (rule ccorresI', erule(5) ccorresE)
   apply simp
   apply (erule rev_bexI)
-  apply (simp add: unif_rrel_def split: split_if_asm)
+  apply (simp add: unif_rrel_def split: if_split_asm)
   apply (cases "hs = []", simp_all)
   done
 
@@ -66,9 +66,9 @@ lemma exec_handlers_Hoare_Post:
   "\<lbrakk> exec_handlers_Hoare \<Gamma> P c Q' A'; Q' \<subseteq> Q; A' \<subseteq> A \<rbrakk>
       \<Longrightarrow> exec_handlers_Hoare \<Gamma> P c Q A"
   apply (simp add: exec_handlers_Hoare_def
-             split del: split_if)
+             split del: if_split)
   apply (elim allEI)
-  apply (simp split: split_if_asm)
+  apply (simp split: if_split_asm)
    apply blast+
   done
 
@@ -96,7 +96,7 @@ lemma exec_handlers_Hoare_from_vcg_might_fail:
   "\<lbrakk> \<Gamma> \<turnstile>\<^bsub>/F\<^esub> P c Q, A; UNIV \<subseteq> A' \<rbrakk> 
     \<Longrightarrow> exec_handlers_Hoare \<Gamma> P (c # hs) Q A'"
   apply (clarsimp simp: exec_handlers_Hoare_def
-             split del: split_if split: split_if_asm)
+             split del: if_split split: if_split_asm)
    apply (erule exec_handlers.cases, simp_all)
     apply (case_tac hsa, simp_all)
      apply (erule exec_handlers.cases, simp_all)
@@ -303,13 +303,13 @@ lemma exec_handlers_Hoare_call_Basic:
   "\<lbrakk> \<forall>s' t x. s' \<in> P \<longrightarrow> g s' t (ret s' t) \<in> Q; UNIV \<subseteq> A \<rbrakk> \<Longrightarrow>
     exec_handlers_Hoare \<Gamma> P (call initfn p ret (\<lambda>x y. Basic (g x y)) # hs) Q A"
   apply (clarsimp simp: exec_handlers_Hoare_def
-             split del: split_if)
+             split del: if_split)
   apply (erule exec_handlers.cases)
     apply clarsimp
     apply (erule exec_call_Normal_elim, simp_all)[1]
      apply (auto elim!: exec_Normal_elim_cases)[1]
     apply (frule exec_handlers_less2, clarsimp+)
-    apply (clarsimp simp: subset_iff split: split_if_asm)
+    apply (clarsimp simp: subset_iff split: if_split_asm)
    apply (auto elim!: exec_Normal_elim_cases
                       exec_call_Normal_elim)
   done
@@ -560,12 +560,12 @@ lemma ccorres_if_lhs:
    \<Longrightarrow> ccorres_underlying sr Gamm r xf arrel axf (\<lambda>s. (P \<longrightarrow> Q s) \<and> (\<not> P \<longrightarrow> R s))
                       {s. (P \<longrightarrow> s \<in> S) \<and> (\<not> P \<longrightarrow> s \<in> T)}
           hs (if P then f else g) conc"
-  by (simp split: split_if)
+  by (simp split: if_split)
 
 lemma ccorres_if_bind:
   "ccorres_underlying sr Gamm r xf arrel axf G G' hs (if a then (b >>= f) else (c >>= f)) d
   \<Longrightarrow> ccorres_underlying sr Gamm r xf arrel axf G G' hs ((if a then b else c) >>= f) d"
-  by (simp split: split_if_asm)
+  by (simp split: if_split_asm)
 
 lemma ccorres_Cond_rhs:
   "\<lbrakk> P \<Longrightarrow> ccorres_underlying sr Gamm rvr xf arrel axf Q S hs absf f;
@@ -667,12 +667,12 @@ lemma ccorres_sequence_while_genQ':
                             (F (n * j)) ({s. xf s = of_nat (i + n * j) \<and> r' ys (xf' s)} \<inter> Q) hs
                             (xs ! n) body"
   and      pn: "\<And>n. P n = (n < of_nat (i + length xs * j))"
-  and   bodyi: "\<forall>s. \<Gamma> \<turnstile>\<^bsub>/UNIV\<^esub> ({s} \<inter> Q) body ({t. xf t = xf s} \<inter> Q)"
+  and   bodyi: "\<forall>s. xf s < of_nat (i + length xs * j)
+    \<longrightarrow> \<Gamma> \<turnstile>\<^bsub>/UNIV\<^esub> ({s} \<inter> Q) body {t. xf t = xf s \<and> xf_update (\<lambda>_. xf t + of_nat j) t \<in> Q}"
   and      hi: "\<And>n. Suc n < length xs \<Longrightarrow> \<lbrace> F (n * j) \<rbrace> (xs ! n) \<lbrace>\<lambda>_. F (Suc n * j)\<rbrace>"
   and     lxs: "i + length xs * j < 2 ^ len_of TYPE('c)"
   and      xf: "\<forall>s f. xf (xf_update f s) = f (xf s) \<and> globals (xf_update f s) = globals s"
   and     xf': "\<forall>s f. xf' (xf_update f s) = (xf' s)"
-  and     xfQ: "\<forall>s f. s \<in> Q \<longrightarrow> xf_update f s \<in> Q"
   and rf_sr_xf: "\<And>s r f. (s, r) \<in> rf_sr \<Longrightarrow> (s, xf_update f r) \<in> rf_sr"
   and       j: " j > 0"
   shows  "ccorresG rf_sr \<Gamma> (\<lambda>rv (i', rv'). r' rv rv' \<and> i' = of_nat (i + length xs * of_nat j))
@@ -772,13 +772,12 @@ proof -
         apply (rule hi''')
         apply simp
        apply (simp add: xf')
-       apply (rule HoarePartialDef.Conseq [where P = "{s. xf s + of_nat j = of_nat (i + (length init_xs - length ys) * of_nat j)} \<inter> Q"])
+       apply (rule HoarePartialDef.Conseq [where P = "{s. P (xf s) \<and> xf s + of_nat j = of_nat (i + (length init_xs - length ys) * of_nat j)} \<inter> Q"])
        apply (intro ballI exI)
-       apply (rule conjI) 
-        apply (rule_tac x = s in spec [OF bodyi])
-       apply (clarsimp simp: xf) 
-       apply (rule xfQ [rule_format])
-       apply simp
+       apply (rule conjI)
+        apply (rule_tac s=s in bodyi[rule_format])
+        apply (clarsimp simp: pn)
+       apply (clarsimp simp: xf)
       apply (clarsimp simp: ln pn')
       apply (subst of_nat_mult [symmetric])+
       apply (subst of_nat_add [symmetric])+
