lib/nicta_lib/sep_algebra/MonadSep.thy
@@ -28,6 +28,7 @@ lemma hoare_gen_lifted_asm:
   by (auto intro: hoare_assume_pre)
 
 lemma mapM_x_sep_inv':
+  includes no_pre
   assumes f:
    "\<And>R x. x \<in> S \<Longrightarrow>
      \<lbrace>\<lambda>s.<P x \<and>* I \<and>* R> s \<and> I' s\<rbrace>
@@ -90,9 +91,9 @@ lemma sep_set_conj_map_singleton_wp:
   \<Longrightarrow> \<lbrace><P \<and>* (\<And>* x\<in>xs. I x) \<and>* R>\<rbrace> f \<lbrace>\<lambda>_. <Q \<and>* (\<And>* x\<in>xs. I x) \<and>* R>\<rbrace>"
   apply (rule hoare_chain [where P="<P \<and>* I x \<and>* (\<And>* x\<in>xs - {x}. I x) \<and>* R>" and
                                  Q="\<lambda>_. <Q \<and>* I x \<and>* (\<And>* x\<in>xs - {x}. I x) \<and>* R>"], assumption)
-   apply (subst (asm) sep.setprod.remove, assumption+)
+   apply (subst (asm) sep.prod.remove, assumption+)
    apply sep_solve
-  apply (subst sep.setprod.remove, assumption+)
+  apply (subst sep.prod.remove, assumption+)
   apply sep_solve
   done
 
